examples/Map.v
@@ -158,7 +158,7 @@ Section MAP.
     Corollary MapInterp_enforce_contract
               (s:    State)
               (Hinv: x_free_map s)
-      : Enforcer (MapInterp s) never_read_x_contract tt.
+      : (MapInterp s) :> never_read_x_contract[tt].
     Proof.
       apply (const_contract_enforcement never_read_x_requirements
                                         never_read_x_promises
@@ -177,7 +177,7 @@ Section MAP.
       [Write k' v].
 
     Lemma read_write_contractful
-      : contractfull_program never_read_x_contract tt read_write.
+      : read_write :> never_read_x_contract[tt].
     Proof.
       unfold read_write.
       constructor.
