theories/Contract/Temporal.v
@@ -98,7 +98,7 @@ Lemma temporal_contract_enforcement
       (Henf: temporal_requirements_enforces_promises step inv promises)
   : forall (s: State),
     inv tl s
-    -> Enforcer (mkInterp step s) (temporal_contract promises) tl.
+    -> (mkInterp step s) :> (temporal_contract promises)[tl].
 Proof.
   intros s Hinv.
   apply (stateful_contract_enforcement (temporal_contract promises)
