theories/Refine.v
@@ -58,7 +58,7 @@ Definition compliant_refinement
          (i: Ii A),
     sync si s so
     -> requirements master i si
-    -> contractfull_program slave so (sr A i s).
+    -> (sr A i s) :> slave[so].
 
 Definition sync_preservation
            {Si So: Type}
@@ -72,7 +72,7 @@ Definition sync_preservation
          (s: S)
          (so: So)
          (int: Interp Io)
-         (Henf: Enforcer int slave so)
+         (Henf: int :> slave[so])
          {A: Type}
          (i: Ii A),
   sync si s so
@@ -93,7 +93,7 @@ Definition sync_promises
          (s: S)
          (so: So)
          (int: Interp Io)
-         (Henf: Enforcer int slave so)
+         (Henf: int :> slave[so])
          {A: Type}
          (i: Ii A),
   sync si s so
@@ -115,9 +115,9 @@ Theorem enforcer_refinement
            (s: S)
            (so: So)
            (int: Interp Io)
-           (Henf: Enforcer int slave so),
+           (Henf: int :> slave[so]),
     sync si s so
-    -> Enforcer (StatefulInterpret sr s int) master si.
+    -> (StatefulInterpret sr s int) :> master[si].
 Proof.
   cofix.
   intros si s so int Henf Hsync.
@@ -130,7 +130,7 @@ Proof.
     apply (Hsyncp si s so int Henf A i Hsync Hreq).
   + intros A i Hreq.
     unfold compliant_refinement in Hcompliant.
-    assert (contractfull_program slave so (sr A i s))
+    assert ((sr A i s) :> slave[so])
       as Hcp
         by  apply (Hcompliant si s so A i Hsync Hreq).
     assert (execInstruction (StatefulInterpret sr s int) i
@@ -145,7 +145,7 @@ Proof.
                                                    so
                                                    (abstract_step slave)
                                                    int).
-       apply (enforcer_contractfull_enforcer _ _ _ int Henf Hcp).
+       apply (enforcer_compliant_enforcer _ _ _ int Henf Hcp).
     ++ apply Hsyncpres.
        +++ exact Henf.
        +++ exact Hsync.
